add fuel to isconf_full and fix other computation issues

safechecker/theories/PCUICSafeConversion.v
@@ -70,6 +70,7 @@ Section Conversion.
   Local Definition hΣ Σ (wfΣ : abstract_env_ext_rel X Σ) :
     ∥ wf Σ ∥ := abstract_env_ext_sq_wf _ _ _ wfΣ. 
 
+  Set Equations Transparent.
   Set Equations With UIP.
 
   Inductive state :=
@@ -488,19 +489,19 @@ Section Conversion.
     intro H. apply ssrbool.introP.
     - intuition.
     - destruct b; intuition.
-  Defined.
+  Qed.
 
   Definition wf_universe_iff  Σ u :
     wf_universeb Σ u <-> wf_universe Σ u.
   Proof.  
     symmetry; apply reflect_iff. eapply wf_universe_reflect.
-  Defined. 
+  Qed. 
 
   Definition wf_universe_instance_iff  Σ u :
     wf_universeb_instance Σ u <-> wf_universe_instance Σ u.
   Proof.  
     symmetry; apply reflect_iff. eapply wf_universe_instanceP.
-  Defined. 
+  Qed. 
 
   Notation conv_stack_ctx Γ π1 π2 :=
     (forall Σ, abstract_env_ext_rel X Σ -> ∥ (Σ ⊢ Γ ,,, stack_context π1 = Γ ,,, stack_context π2) ∥).
@@ -1587,7 +1588,7 @@ Qed.
     + eapply red_const. erewrite abstract_env_lookup_correct; eauto.
     + specialize (hx _ wfΣ). clear -hx wΣ. sq.  fvs. 
     Unshelve. all : eauto. 
-  Defined. 
+  Qed. 
   Next Obligation.
     (* Contraposition of previous goal *)
     apply h; clear h. intros Σ wfΣ. 
@@ -1600,7 +1601,7 @@ Qed.
     + eapply red_const. erewrite abstract_env_lookup_correct; eauto.
     + specialize (hx _ wfΣ). sq; fvs. 
     Unshelve. eauto. 
-  Defined. 
+  Qed. 
   Next Obligation.
     (* Both c and c' are axioms. Either they are different constants or they are not
        convertible because the universes are different. *)
@@ -1627,22 +1628,22 @@ Qed.
     eapply eqb_universe_instance_complete in r; auto.
   Qed.
   (* Why Solve All Obligations is not working here ??? *)
-  Next Obligation. solve_unfold_constants aux eq1 eq2 Σ wfΣ. Defined. 
-  Next Obligation. solve_unfold_constants aux eq1 eq2 Σ wfΣ. Defined. 
-  Next Obligation. solve_unfold_constants aux eq1 eq2 Σ wfΣ. Defined. 
-  Next Obligation. solve_unfold_constants aux eq1 eq2 Σ wfΣ. Defined. 
-  Next Obligation. solve_unfold_constants aux eq1 eq2 Σ H. Defined. 
-  Next Obligation. solve_unfold_constants aux eq1 eq2 Σ wfΣ. Defined. 
-  Next Obligation. solve_unfold_constants aux eq1 eq2 Σ wfΣ. Defined. 
-  Next Obligation. solve_unfold_constants aux eq1 eq2 Σ wfΣ. Defined. 
-  Next Obligation. solve_unfold_constants aux eq1 eq2 Σ wfΣ. Defined. 
-  Next Obligation. solve_unfold_constants aux eq1 eq2 Σ wfΣ. Defined. 
-  Next Obligation. solve_unfold_constants aux eq1 eq2 Σ wfΣ. Defined. 
-  Next Obligation. solve_unfold_constants aux eq1 eq2 Σ H. Defined. 
-  Next Obligation. solve_unfold_constants aux eq1 eq2 Σ wfΣ. Defined. 
-  Next Obligation. solve_unfold_constants aux eq1 eq2 Σ wfΣ. Defined. 
-  Next Obligation. solve_unfold_constants aux eq1 eq2 Σ wfΣ. Defined. 
-  Next Obligation. solve_unfold_constants aux eq1 eq2 Σ wfΣ. Defined. 
+  Next Obligation. solve_unfold_constants aux eq1 eq2 Σ wfΣ. Qed. 
+  Next Obligation. solve_unfold_constants aux eq1 eq2 Σ wfΣ. Qed. 
+  Next Obligation. solve_unfold_constants aux eq1 eq2 Σ wfΣ. Qed. 
+  Next Obligation. solve_unfold_constants aux eq1 eq2 Σ wfΣ. Qed. 
+  Next Obligation. solve_unfold_constants aux eq1 eq2 Σ H. Qed. 
+  Next Obligation. solve_unfold_constants aux eq1 eq2 Σ wfΣ. Qed. 
+  Next Obligation. solve_unfold_constants aux eq1 eq2 Σ wfΣ. Qed. 
+  Next Obligation. solve_unfold_constants aux eq1 eq2 Σ wfΣ. Qed. 
+  Next Obligation. solve_unfold_constants aux eq1 eq2 Σ wfΣ. Qed. 
+  Next Obligation. solve_unfold_constants aux eq1 eq2 Σ wfΣ. Qed. 
+  Next Obligation. solve_unfold_constants aux eq1 eq2 Σ wfΣ. Qed. 
+  Next Obligation. solve_unfold_constants aux eq1 eq2 Σ H. Qed. 
+  Next Obligation. solve_unfold_constants aux eq1 eq2 Σ wfΣ. Qed. 
+  Next Obligation. solve_unfold_constants aux eq1 eq2 Σ wfΣ. Qed. 
+  Next Obligation. solve_unfold_constants aux eq1 eq2 Σ wfΣ. Qed. 
+  Next Obligation. solve_unfold_constants aux eq1 eq2 Σ wfΣ. Qed. 
   
   Lemma welltyped_zipc_tCase_brs_length Σ (wfΣ : abstract_env_ext_rel X Σ) Γ ci motive discr brs π :
     welltyped Σ Γ (zipc (tCase ci motive discr brs) π) ->
@@ -1734,7 +1735,7 @@ Qed.
     pose proof (heΣ _ wfΣ). specialize (cc _ wfΣ). sq. 
     constructor; fvs. 
     - constructor.
-  Defined.
+  Qed.
   Next Obligation.
     destruct (abstract_env_ext_exists X) as [[Σ wfΣ]]; 
     pose proof (hΣ _ wfΣ). specialize (H _ wfΣ). sq.
@@ -2056,7 +2057,7 @@ Qed.
       eapply proof_irrelevance.
     }
     rewrite <- e. assumption.
-  Qed. 
+  Defined. 
   Next Obligation.
     destruct (case_conv_brs_inv h p' c' brs1' brs2' _ h') as [[mdecl [idecl [decli eqp eqp' eqm clm clm']]]]; tea.
     specialize_Σ wfΣ. 
@@ -2101,7 +2102,7 @@ Qed.
   Qed.
   Next Obligation.
     unshelve eapply aux. all: eassumption.
-  Qed.
+  Defined.
 
   (* Factorise notions of fixpoints *)
   Inductive fix_kind :=
@@ -2267,7 +2268,7 @@ Qed.
       eapply proof_irrelevance.
     }
     rewrite <- e. assumption.
-  Qed.
+  Defined.
   Next Obligation.
     destruct (abstract_env_ext_exists X) as [[Σ wfΣ]].
     specialize_Σ wfΣ.
@@ -2488,7 +2489,7 @@ Qed.
       + eapply IHh.
       + eapply r0. 2:lia.
         clear - wΣ IHh. fvs. 
-  Defined. 
+  Qed. 
   Next Obligation.
     rewrite <- app_assoc. simpl. eauto.
   Qed.
@@ -2547,7 +2548,7 @@ Qed.
       eapply proof_irrelevance.
     }
     rewrite <- e. assumption.
-  Qed.
+  Defined.
   Next Obligation.
     destruct (abstract_env_ext_exists X) as [[Σ wfΣ]].
     specialize_Σ wfΣ.
@@ -2620,10 +2621,10 @@ Qed.
 
   Next Obligation.
     unshelve eapply aux. all: eassumption.
-  Qed.
+  Defined.
   Next Obligation.
     unshelve eapply aux. all: eassumption.
-  Qed.
+  Defined.
   Next Obligation.
     destruct h1 as [h1], h2 as [h2].
     constructor.
@@ -3192,14 +3193,11 @@ Qed.
       1:now eapply ws_cumul_ctx_pb_closed_left in hx.
       eapply on_free_vars_ctx_inst_case_context; trea.
       fvs.
-(*    - eapply eqb_universe_instance_spec in eq_insts; eauto. 
-      destruct (case_conv_preds_inv _ wfΣ h1 _ _ _ h2 hx eq_insts (conv_params Σ wfΣ)) as []; tea.
-     *)
      - destruct (case_conv_preds_inv _ wfΣ h1 _ _ _ h2 hx (conv_params Σ wfΣ)) as []; tea.
        destruct X1 as [mdecl [idecl []]]. eauto. 
      - destruct (case_conv_preds_inv _ wfΣ h1 _ _ _ h2 hx (conv_params Σ wfΣ)) as []; tea.
        destruct X1 as [mdecl [idecl []]]. eauto. 
-  Defined.
+  Qed.
   Next Obligation.
     unfold zipp in conv_ret; simpl in conv_ret.
     destruct (case_conv_preds_inv _ wfΣ h1 _ _ _ h2 hx (conv_params Σ wfΣ)) as []; tea. 
@@ -3211,7 +3209,7 @@ Qed.
     now destruct X0 as [mdecl [idecl []]].
     - now destruct X0 as [mdecl [idecl []]].
     - now destruct X0 as [mdecl [idecl []]].
-  Defined.
+  Qed.
   Next Obligation.
     unfold zipp in not_conv_ret; simpl in not_conv_ret.
     contradiction not_conv_ret.
@@ -4665,20 +4663,21 @@ Qed.
     split. 1: reflexivity.
     rewrite !stack_position_cons.
     eapply positionR_poscat. constructor.
-  Defined.
+  Qed.
   Next Obligation.
     rewrite 2!stack_context_appstack.
     eauto.
   Qed.
   Next Obligation.
     rewrite mkApps_app. eauto.
-  Defined.
+  Qed.
   Next Obligation.
-    simpl in H0. destruct H0 as [eq hp].
-    rewrite app_length in H. cbn in H.
     eapply aux. all: auto.
-    - cbn. lia.
-    - instantiate (1 := h2'). simpl. split.
+    - cbn. simpl in H0. destruct H0 as [eq hp].
+      rewrite app_length in H. cbn in H. lia.
+    - instantiate (1 := h2'). simpl in H0. destruct H0 as [eq hp].
+      rewrite app_length in H. cbn in H.
+      simpl. split.
       + rewrite mkApps_app in eq. assumption.
       + subst x y.
         rewrite !stack_position_cons, !stack_position_appstack.
@@ -4703,7 +4702,7 @@ Qed.
     rewrite stack_context_appstack in H1.
     destruct H2 as [H2].
     constructor; constructor; auto.
-  Defined.
+  Qed.
   Next Obligation.
     apply herr; clear herr. intros Σ wfΣ. specialize_Σ wfΣ.
     destruct H as [H]; depelim H.
@@ -4753,14 +4752,13 @@ Qed.
     eauto.
   Qed.
   Next Obligation.
-    specialize (aux Reduction) as h. cbn in h.
-    eapply h. all: auto.
+    eapply (aux Reduction). all: auto.
     pose proof (decompose_stack_eq _ _ _ (eq_sym eq1)). subst.
     instantiate (1 := h2').
     simpl in H0. destruct H0 as [eq hp].
     unshelve eapply R_positionR. 2: assumption.
     simpl. rewrite eq. reflexivity.
-  Qed.
+  Defined.
   (* The obligation tactic wipes out a useful hypothesis here? *)
   Obligation Tactic := idtac.
   Next Obligation.
@@ -5718,16 +5716,30 @@ Qed.
     _isconv Fallback Γ t1 π1 h1 t2 π2 h2 aux :=
       λ { | leq | hx | r1 | r2 | hd := _isconv_fallback Γ leq t1 π1 h1 t2 π2 h2 r1 r2 hd hx aux }.
 
+    Lemma welltyped_R_zipc Σ (wfΣ : abstract_env_ext_rel X Σ) Γ :
+      forall x y : pack Γ, welltyped Σ Γ (zipc (tm1 x) (stk1 x)) -> R Γ y x -> welltyped Σ Γ (zipc (tm1 y) (stk1 y)).
+    Proof.
+      intros x y H HR.
+      pose proof (heΣ := heΣ _ wfΣ).
+      pose proof (hΣ := hΣ _ wfΣ). cbn.
+      sq. 
+      destruct x, y; cbn in *.
+      (* dependent induction HR.
+      - eapply cored_welltyped. all: eauto.
+        cbn in *. specialize_Σ wfΣ. destruct H.
+      - simpl in H1. revert H1; intros [= H2 _].
+        now rewrite <- H2. *)
+    Admitted.
+
   Equations(noeqns) isconv_full (s : state) (Γ : context)
             (t1 : term) (π1 : stack) (h1 : wtp Γ t1 π1)
             (t2 : term) (π2 : stack) (h2 : wtp Γ t2 π2)
     : Ret s Γ t1 π1 t2 π2 :=
 
-    isconv_full s Γ t1 π1 h1 t2 π2 h2 hx :=
+    isconv_full s Γ t1 π1 h1 t2 π2 h2 hx _ :=
       Fix_F (R := R Γ)
             (fun '(mkpack s' t1' π1' t2' π2' h2') =>
               wtp Γ t1' π1' ->
-              wtp Γ t2' π2' ->
               Ret s' Γ t1' π1' t2' π2'
             )
             (fun pp f => _)
@@ -5735,15 +5747,25 @@ Qed.
             _ _ _ _.
   Next Obligation.
     unshelve eapply _isconv. all: try assumption.
-    intros s' t1' π1' t2' π2' h1' h2' hx' hR.
-    destruct pp.
-    assert (wth0 = H0) by apply proof_irrelevance. simpl in hR. subst.
-    specialize (f (mkpack Γ s' t1' π1' t2' π2' h2') hR). cbn in f.
-    eapply f ; assumption.
-  Qed.
+    - destruct pp; cbn in *; eauto.
+    - intros s' t1' π1' t2' π2' h1' h2' hx' hR.
+    specialize (f (mkpack Γ s' t1' π1' t2' π2' h2') hR).
+    eapply f ; try assumption.
+  Defined.
   Next Obligation.
-    apply R_Acc. assumption.
-  Qed.
+  match goal with | |- Acc _ ?X => set (u := X) end.
+  revert h1.  
+  change ((forall Σ, abstract_env_ext_rel X Σ -> welltyped Σ Γ (zipc (tm1 u) (stk1 u))) -> Acc (R Γ) u).
+  generalize u.
+  refine (Acc_intro_generator
+            (R:=R Γ)
+            (P:=fun u => forall Σ (wfΣ : abstract_env_ext_rel X Σ), welltyped Σ Γ (zipc (tm1 u) (stk1 u)))
+            (fun x y Px Hy => _) 1000 _); intros.
+  - simpl in *. eapply welltyped_R_zipc; eauto.
+  - destruct (abstract_env_ext_exists X) as [[Σ wfΣ]].
+    destruct (hΣ _ wfΣ) as [hΣ]. eapply R_Acc; eassumption.
+  Defined.
+
   
   Inductive ConversionResultSummary :=
   | ConvSuccess : ConversionResultSummary
@@ -5788,7 +5810,7 @@ Qed.
     destruct (h1 _ H), (hΣ _ H) as [wΣ].
     sq. eapply ws_cumul_ctx_pb_refl. 
     fvs.
-  Defined.
+  Qed.
   
   Theorem isconv_term_sound :
     forall Σ (wfΣ : abstract_env_ext_rel X Σ) Γ leq t1 h1 t2 h2,
@@ -5812,3 +5834,34 @@ Qed.
   Transparent reduce_stack.
   
 End Conversion.
+
+(*
+From MetaCoq.SafeChecker Require Import PCUICWfEnvImpl.
+Definition default_normal : @normalizing_flags default_checker_flags.
+now econstructor.
+Defined.
+
+Lemma test_conv :
+match
+  isconv_term (cf := default_checker_flags) 
+    (nor := default_normal)
+     canonical_abstract_env_ext_impl
+    {|
+      referenced_impl_env_ext :=
+        ({|
+           universes :=
+             (LevelSet.add Level.lzero LevelSet.empty, ConstraintSet.empty);
+           declarations := []
+         |}, Monomorphic_ctx);
+      referenced_impl_ext_wf := todo "foo"
+    |} [] Cumul (tSort (Universe.lType (Universe.make' (Level.lzero, 0))))
+    (todo "") (tSort (Universe.lType (Universe.make' (Level.lzero, 0))))
+    (todo "")
+with
+| ConvSuccess => "success"
+| ConvError _ => todo "foo"
+end = "success".
+Proof.
+  lazy. reflexivity.
+Defined.
+*)
